All before Shrink

specs/P256.S.fst
@@ -9,7 +9,7 @@ open Spec.Lib
 open Spec.Lib.IntBuf
 open Spec.Lib.IntTypes
 
-
+open Spec.Lib.IntSeq.Lemmas
 
 module Buffer = Spec.Lib.IntBuf
 
@@ -19,8 +19,6 @@ let nlimbs' = 4ul
 
 (* Type aliases *)
 type limb = uint128
-
-
 type felem = lbuffer limb nlimbs
 type longfelem = lbuffer limb (2 * nlimbs)
 type smallfelem = lbuffer uint64 nlimbs
@@ -53,7 +51,11 @@ val kPrime: unit ->
     (ensures (fun h0 b h1 -> True))
 
 let kPrime () = 
-	let b = createL [(u64(0xffffffffffffffff)); (u64(0xffffffff)); (u64(0x0)); (u64(0xffffffff00000001))] in 
+	let b = create_smallfelem() in 
+	upd b 0 (u64(0xffffffffffffffff)); 
+	upd b 1 (u64(0xffffffff)); 
+	upd b 2 (u64(0x0));
+	upd b 3 (u64(0xffffffff00000001));
 	b	
 
 
@@ -258,43 +260,3 @@ let longfelem_scalar out scalar =
   out.(5) <- mul_wide o5 scalar;
   out.(6) <- mul_wide o6 scalar;
   out.(7) <- mul_wide o7 scalar
-
-(*)
-val load128: high: (uint_t U64) -> low: (uint_t U64) -> 
-    Pure (uint_t U128) (requires True) 
-    (ensures (fun b ->uint_v b = pow2 64 * uint_v high + uint_v low ))
-
-let load128 high low = 
-    let high = to_u128(high) in 
-    let shift = u32(64) in 
-    let hs = shift_left high shift in 
-    	assert (uint_v hs = pow2 64 * uint_v high); 
-    let ls = to_u128(low) in 
-    	assert(uint_v ls = uint_v low);
-    let result = logor hs ls in 
-    	assert(uint_v (logor hs ls) = uint_v hs + uint_v ls);
-    	assume (uint_v result = pow2 64 * uint_v high + uint_v low);
-    result
-(*)
-let two105m41m9 = load128 (u64(0x1ffffffffff)) (u64(0xfffffdfffffffe00))
-let two105      = load128 (u64(0x30000000000)) (u64(0x0))
-let two105m41p9 = load128 (u64(0x1ffffffffff)) (u64(0xfffffe0000000200))
-
-let two107m43m11 = load128 (u64(0x7ffffffffff)) (u64(0xfffff7fffffff800))
-let two107       = load128 (u64(0x80000000000)) (u64(0x0))
-let two107m43p11 = load128 (u64(0x7ffffffffff)) (u64(0xfffff80000000800))
-
-let two64m0     =  to_u128 (u64(0xffffffffffffffff))
-let two110p32m0 = load128 (u64(0x400000000000)) (u64(0x00000000ffffffff))
-let two64m46    = to_u128 (u64(0xffffc00000000000))
-let two64m32    = to_u128 (u64(0xffffffff00000000))
-
-let two70m8p6     = load128 (u64(0x3f)) (u64(0xffffffffffffff40))
-let two70p40      = load128 (u64(0x40)) (u64(0x0000010000000000))
-let two70         = load128  (u64(0x40)) (u64(0x0000010000000000))
-let two70m40m38p6 = load128 (u64(0x3f)) (u64(0xfffffec000000040))
-let two70m6       = load128 (u64(0x3f)) (u64(0xffffffffffffffc0))
-
-let two100m36m4 = load128 (u64(0xfffffffff)) (u64(0xffffffeffffffff0))
-let two100      = load128 (u64(0x1000000000)) (u64(0x0))
-let two100m36p4 = load128 (u64(0xfffffffff)) (u64(0xfffffff000000010))
