specs/Hacl.P256.SmallNegation.fst
@@ -1,0 +1,245 @@
+module Hacl.P256.SmallNegation
+
+open FStar.Mul
+
+open FStar.HyperStack
+open FStar.HyperStack.ST
+
+open Spec.Lib
+open Spec.Lib.IntSeq
+open Spec.Lib.IntBuf
+open Spec.Lib.IntTypes
+open Spec.Lib.IntSeq.Lemmas
+
+open P256.S
+open Hacl.P256.Zeros
+
+#set-options " --z3rlimit 200 "
+
+
+val smallfelem_neg: out:felem -> small:smallfelem ->tempBuffer: felem ->  Stack unit
+  (requires (fun h -> live h out /\ live h small /\ live h tempBuffer))
+  (ensures (fun h0 _ h1 -> preserves_live h0 h1 /\ modifies2 out tempBuffer h0 h1 )) (* /\ modifies1 out h0 h1*)
+
+let smallfelem_neg out small tempBuffer =
+	zero105_2 tempBuffer;
+	let small0 = small.(0) in
+	let small1 = small.(1) in
+	let small2 = small.(2) in
+	let small3 = small.(3) in
+	let zero0  = tempBuffer.(0) in
+	let zero1  = tempBuffer.(1) in
+	let zero2  = tempBuffer.(2) in
+	let zero3  = tempBuffer.(3) in
+		assert((uint_v zero0) >= (uint_v small0));
+		assert((uint_v zero1) >= (uint_v small1));
+		assert((uint_v zero2) >= (uint_v small2));
+		assert((uint_v zero3) >= (uint_v small3));
+	out.(0) <- sub zero0 (to_u128 (small0));
+	out.(1) <- sub zero0 (to_u128 (small1));
+	out.(2) <- sub zero0 (to_u128 (small2));
+	out.(3) <- sub zero0 (to_u128 (small3))
+
+
+val felem_diff: out:felem -> input:felem -> 
+	tempBuffer: felem -> Stack unit
+    (requires (fun h -> live h out /\ live h input /\ live h tempBuffer /\
+     	disjoint out tempBuffer /\ disjoint input tempBuffer /\
+     	(let input = as_lseq input h in 
+     		let input0 = Spec.Lib.IntSeq.index input 0 in 
+     		let input1 = Spec.Lib.IntSeq.index input 1 in 
+     		let input2 = Spec.Lib.IntSeq.index input 2 in 
+     		let input3 = Spec.Lib.IntSeq.index input 3 in 
+     		uint_v input0 < pow2 104 /\
+     		uint_v input1 < pow2 104 /\
+     		uint_v input2 < pow2 104 /\
+     		uint_v input3 < pow2 104 
+     	)
+     	/\
+    	(let out = as_lseq out h in 
+    	let out0 = Spec.Lib.IntSeq.index out 0 in 
+    	let out1 = Spec.Lib.IntSeq.index out 1 in 
+    	let out2 = Spec.Lib.IntSeq.index out 2 in 
+    	let out3 = Spec.Lib.IntSeq.index out 3 in 
+     	uint_v out0 < pow2 128 - (uint_v two105m41m9) /\
+    	uint_v out1 < pow2 128 - (uint_v two105) /\
+		uint_v out2 < pow2 128 - (uint_v two105m41p9) /\
+		uint_v out3 < pow2 128 - (uint_v two105m41p9)
+				))
+	)
+    (ensures (fun h0 _ h1 -> preserves_live h0 h1 /\ modifies2 tempBuffer out h0 h1))
+
+#set-options " --z3rlimit 500 "
+
+let felem_diff out input tempBuffer=
+zero105_2 tempBuffer;
+  let input0 = input.(0) in
+  let input1 = input.(1) in
+  let input2 = input.(2) in
+  let input3 = input.(3) in
+	let out0 = index out 0 in 
+	let out1 = index out 1 in 
+	let out2 = index out 2 in 
+	let out3 = index out 3 in 
+  let zero0  = tempBuffer.(0) in
+  let zero1  = tempBuffer.(1) in
+  let zero2  = tempBuffer.(2) in 
+  let zero3  = tempBuffer.(3) in
+  let out0 = add zero0 out0 in
+  let out1 = add zero1 out1 in
+  let out2 = add zero2 out2 in
+  let out3 = add zero3 out3 in
+	  assert_norm (uint_v two105m41m9 > pow2 104);
+	  assert_norm (uint_v two105 > pow2 104);
+	  assert_norm (uint_v two105m41p9 > pow2 104);
+  out.(0) <- sub out0 input0;
+  out.(1) <- sub out1 input1;
+  out.(2) <- sub out2 input2;
+  out.(3) <- sub out3 input3
+ 
+
+
+val felem_diff_zero107:
+  out:felem -> input:felem -> 
+	tempBuffer: felem -> Stack unit
+    (requires (fun h -> live h out /\ live h input /\ live h tempBuffer /\
+     	disjoint out tempBuffer /\ disjoint input tempBuffer /\
+     	(let input = as_lseq input h in 
+     		let input0 = Spec.Lib.IntSeq.index input 0 in 
+     		let input1 = Spec.Lib.IntSeq.index input 1 in 
+     		let input2 = Spec.Lib.IntSeq.index input 2 in 
+     		let input3 = Spec.Lib.IntSeq.index input 3 in 
+     		uint_v input0 < pow2 106 /\
+     		uint_v input1 < pow2 106 /\
+     		uint_v input2 < pow2 106 /\
+     		uint_v input3 < pow2 106 
+     	)
+     	/\
+    	(let out = as_lseq out h in 
+    	let out0 = Spec.Lib.IntSeq.index out 0 in 
+    	let out1 = Spec.Lib.IntSeq.index out 1 in 
+    	let out2 = Spec.Lib.IntSeq.index out 2 in 
+    	let out3 = Spec.Lib.IntSeq.index out 3 in 
+     	uint_v out0 < pow2 128 - (uint_v two107m43m11) /\
+    	uint_v out1 < pow2 128 - (uint_v two107) /\
+		uint_v out2 < pow2 128 - (uint_v two107m43p11) /\
+		uint_v out3 < pow2 128 - (uint_v two107m43p11)
+				))
+	)
+    (ensures (fun h0 _ h1 -> preserves_live h0 h1 /\ modifies2 tempBuffer out h0 h1))
+
+
+let felem_diff_zero107 out input tempBuffer=
+zero107_2 tempBuffer;
+  let input0 = input.(0) in
+  let input1 = input.(1) in
+  let input2 = input.(2) in
+  let input3 = input.(3) in
+	let out0 = index out 0 in 
+	let out1 = index out 1 in 
+	let out2 = index out 2 in 
+	let out3 = index out 3 in 
+  let zero0  = tempBuffer.(0) in
+  let zero1  = tempBuffer.(1) in
+  let zero2  = tempBuffer.(2) in 
+  let zero3  = tempBuffer.(3) in
+  let out0 = add zero0 out0 in
+  let out1 = add zero1 out1 in
+  let out2 = add zero2 out2 in
+  let out3 = add zero3 out3 in
+	  assert_norm (uint_v two107m43m11 > pow2 106);
+	  assert_norm (uint_v two107 > pow2 106);
+	  assert_norm (uint_v two107m43p11 > pow2 106);
+  out.(0) <- sub out0 input0;
+  out.(1) <- sub out1 input1;
+  out.(2) <- sub out2 input2;
+  out.(3) <- sub out3 input3
+
+val longfelem_diff:
+  out:longfelem -> input:longfelem ->
+   Stack unit
+    (requires (fun h -> live h out /\ live h input 
+    	 /\
+     	(let input = as_lseq input h in 
+     		let input0 = Spec.Lib.IntSeq.index input 0 in 
+     		let input1 = Spec.Lib.IntSeq.index input 1 in 
+     		let input2 = Spec.Lib.IntSeq.index input 2 in 
+     		let input3 = Spec.Lib.IntSeq.index input 3 in 
+     		let input4 = Spec.Lib.IntSeq.index input 4 in 
+     		let input5 = Spec.Lib.IntSeq.index input 5 in 
+     		let input6 = Spec.Lib.IntSeq.index input 6 in 
+     		let input7 = Spec.Lib.IntSeq.index input 7 in 
+     		uint_v input0 < 7 * pow2 67 /\
+     		uint_v input1 < 7 * pow2 67 /\
+     		uint_v input2 < 7 * pow2 67 /\
+     		uint_v input3 < 7 * pow2 67 /\
+     		uint_v input4 < 7 * pow2 67 /\
+     		uint_v input5 < 7 * pow2 67 /\
+     		uint_v input6 < 7 * pow2 67 /\
+     		uint_v input7 < 7 * pow2 67 
+     	)	
+    	/\
+    	(let out = as_lseq out h in 
+    	let out0 = Spec.Lib.IntSeq.index out 0 in 
+    	let out1 = Spec.Lib.IntSeq.index out 1 in 
+    	let out2 = Spec.Lib.IntSeq.index out 2 in 
+    	let out3 = Spec.Lib.IntSeq.index out 3 in 
+		let out4 = Spec.Lib.IntSeq.index out 4 in 
+		let out5 = Spec.Lib.IntSeq.index out 5 in 
+		let out6 = Spec.Lib.IntSeq.index out 6 in 
+		let out7 = Spec.Lib.IntSeq.index out 7 in 
+     	uint_v out0 < pow2 128 - (uint_v two70m8p6) /\
+    	uint_v out1 < pow2 128 - (uint_v two70p40) /\
+		uint_v out2 < pow2 128 - (uint_v two70) /\
+		uint_v out3 < pow2 128 - (uint_v two70m40m38p6) /\
+		uint_v out4 < pow2 128 - (uint_v two70m6) /\
+		uint_v out5 < pow2 128 - (uint_v two70m6) /\
+		uint_v out6 < pow2 128 - (uint_v two70m6) /\
+		uint_v out7 < pow2 128 - (uint_v two70m6) 
+	)
+
+    ))
+    (ensures (fun h0 _ h1 -> preserves_live h0 h1 /\ modifies1 out h0 h1))
+
+let longfelem_diff out input =
+  let input0 = input.(0) in
+  let input1 = input.(1) in
+  let input2 = input.(2) in
+  let input3 = input.(3) in
+  let input4 = input.(4) in
+  let input5 = input.(5) in
+  let input6 = input.(6) in
+  let input7 = input.(7) in
+  let out0 = out.(0) in
+  let out1 = out.(1) in
+  let out2 = out.(2) in
+  let out3 = out.(3) in
+  let out4 = out.(4) in
+  let out5 = out.(5) in
+  let out6 = out.(6) in
+  let out7 = out.(7) in
+  let out0 = add two70m8p6 out0 in
+  let out1 = add two70p40 out1 in
+  let out2 = add two70 out2 in
+  let out3 = add two70m40m38p6 out3 in
+  let out4 = add two70m6 out4 in
+  let out5 = add two70m6 out5 in
+  let out6 = add two70m6 out6 in
+  let out7 = add two70m6 out7 in
+
+	assert_norm(uint_v two70m8p6 > pow2 70 - pow2 40 - pow2 38);
+	assert_norm(uint_v two70p40 >  pow2 70 - pow2 40 - pow2 38);
+	assert_norm(uint_v two70 >  pow2 70 - pow2 40 - pow2 38);
+	assert_norm(uint_v two70m40m38p6 >  pow2 70 - pow2 40 - pow2 38);
+	assert_norm(uint_v two70m6 >  pow2 70 - pow2 40 - pow2 38);
+
+	assert_norm(7 * pow2 67 <  pow2 70 - pow2 40 - pow2 38);	
+
+  out.(0) <- sub out0 input0;
+  out.(1) <- sub out1 input1;
+  out.(2) <- sub out2 input2;
+  out.(3) <- sub out3 input3;
+  out.(4) <- sub out4 input4;
+  out.(5) <- sub out5 input5;
+  out.(6) <- sub out6 input6;
+  out.(7) <- sub out7 input7
